Finished updating safechecker (some todos left)

safechecker/theories/PCUICTypeChecker.v
@@ -92,6 +92,15 @@ Section Typecheck.
     assumption.
   Qed.
 
+
+  Definition wt_decl (Σ : global_env_ext) Γ d :=
+    match d with
+    | {| decl_body := Some b; decl_type := ty |} => 
+      welltyped Σ Γ ty /\ welltyped Σ Γ b
+    | {| decl_body := None; decl_type := ty |} =>
+      welltyped Σ Γ ty
+    end.
+
   Section InferAux.
     Variable (infer : forall Γ (HΓ : ∥ wf_local Σ Γ ∥) (t : term),
                  typing_result ({ A : term & ∥ Σ ;;; Γ |- t : A ∥ })).
@@ -107,6 +116,13 @@ Section Typecheck.
     Next Obligation.
       destruct HΣ, HΓ, X, X0.
       now constructor; eapply type_reduction.
+    Defined.
+
+    Program Definition infer_isType Γ HΓ T : typing_result (∥ isType Σ Γ T ∥) :=
+      tx <- infer_type Γ HΓ T ;;
+      ret _.
+    Next Obligation.
+      sq. now eexists.
     Defined.
 
     Program Definition infer_cumul Γ HΓ t A (hA : ∥ isType Σ Γ A ∥)
@@ -139,6 +155,307 @@ Section Typecheck.
       sq.
       eapply type_reduction; eauto.
     Qed.
+
+    Lemma sq_wfl_nil : ∥ wf_local Σ [] ∥.
+    Proof.
+     repeat constructor.
+    Qed.
+
+    Program Fixpoint check_context Γ : typing_result (∥ wf_local Σ Γ ∥)
+    := match Γ with
+       | [] => ret sq_wfl_nil
+       | {| decl_body := None; decl_type := A |} :: Γ =>
+         HΓ <- check_context Γ ;;
+         XX <- infer_type Γ HΓ A ;;
+         ret _
+       | {| decl_body := Some t; decl_type := A |} :: Γ =>
+         HΓ <- check_context Γ ;;
+         XX <- infer_type Γ HΓ A ;;
+         XX <- infer_cumul Γ HΓ t A _ ;;
+         ret _
+      end.
+    Next Obligation.
+      sq. econstructor; tas. econstructor; eauto.
+    Qed.
+    Next Obligation.
+      sq. econstructor; tea.
+    Qed.
+    Next Obligation.
+      sq. econstructor; tas. econstructor; eauto.
+    Qed.
+ 
+    Lemma sq_wf_locak_app {Γ Δ} : ∥ wf_local Σ Γ ∥ -> ∥ wf_local_rel Σ Γ Δ ∥ -> ∥ wf_local Σ (Γ ,,, Δ) ∥.
+    Proof.
+      intros [] []; constructor; now apply wf_local_app.
+    Qed. 
+
+    Program Fixpoint check_context_rel Γ (Δ : context) :
+      ∥ wf_local Σ Γ ∥ -> typing_result (∥ wf_local_rel Σ Γ Δ ∥) :=
+      match Δ return ∥ wf_local Σ Γ ∥ -> typing_result (∥ wf_local_rel Σ Γ Δ ∥) with
+       | [] => fun wfΓ => ret (sq localenv_nil)
+       | {| decl_body := None; decl_type := A |} :: Δ =>
+        fun wfΓ =>
+         wfΔ <- check_context_rel Γ Δ wfΓ ;;
+         XX <- infer_isType (Γ ,,, Δ) (sq_wf_locak_app wfΓ wfΔ) A ;;
+         ret _
+       | {| decl_body := Some t; decl_type := A |} :: Δ =>
+         fun wfΓ => 
+         wfΔ <- check_context_rel Γ Δ wfΓ ;;
+         Aty <- infer_isType (Γ ,,, Δ) (sq_wf_locak_app wfΓ wfΔ) A ;;
+         XX <- infer_cumul (Γ ,,, Δ) (sq_wf_locak_app wfΓ wfΔ) t A Aty ;;
+         ret _
+      end.
+    Next Obligation.
+      sq. constructor; auto.
+    Qed.
+    Next Obligation.
+      sq. constructor; auto.
+    Qed.
+
+    Program Definition check_cumul_decl Γ d d' : wt_decl Σ Γ d -> wt_decl Σ Γ d' -> typing_result (∥ cumul_decls Σ Γ Γ d d' ∥) := 
+      match d, d' return wt_decl Σ Γ d -> wt_decl Σ Γ d' -> typing_result _ with
+      | {| decl_name := na; decl_body := Some b; decl_type := ty |},
+        {| decl_name := na'; decl_body := Some b'; decl_type := ty' |} => 
+        fun wtd wtd' =>
+        eqna <- check_eq_true (eqb_binder_annot na na') (Msg "Binder annotations do not match") ;;
+        cumb <- convert Γ b b' _ _ ;;
+        cumt <- convert_leq Γ ty ty' _ _ ;;
+        ret (let 'sq cumb := cumb in 
+              let 'sq cumt := cumt in
+              sq _)
+      | {| decl_name := na; decl_body := None; decl_type := ty |},
+        {| decl_name := na'; decl_body := None; decl_type := ty' |} => 
+        fun wtd wtd' =>
+        eqna <- check_eq_true (eqb_binder_annot na na') (Msg "Binder annotations do not match") ;;
+        cumt <- convert_leq Γ ty ty' wtd wtd' ;;
+        ret (let 'sq cumt := cumt in sq _)      
+      | _, _ =>
+        fun wtd wtd' => raise (Msg "While checking cumulativity of contexts: declarations do not match")
+      end.
+    Next Obligation.
+      constructor; pcuics. now apply eqb_binder_annot_spec.
+    Qed.
+    Next Obligation.
+      constructor; pcuics. now apply eqb_binder_annot_spec.
+    Qed.
+
+    Program Definition check_conv_decl Γ d d' : wt_decl Σ Γ d -> wt_decl Σ Γ d' -> typing_result (∥ conv_decls Σ Γ Γ d d' ∥) := 
+      match d, d' return wt_decl Σ Γ d -> wt_decl Σ Γ d' -> typing_result _ with
+      | {| decl_name := na; decl_body := Some b; decl_type := ty |},
+        {| decl_name := na'; decl_body := Some b'; decl_type := ty' |} => 
+        fun wtd wtd' =>
+        eqna <- check_eq_true (eqb_binder_annot na na') (Msg "Binder annotations do not match") ;;
+        cumb <- convert Γ b b' _ _ ;;
+        cumt <- convert Γ ty ty' _ _ ;;
+        ret (let 'sq cumb := cumb in 
+              let 'sq cumt := cumt in
+              sq _)
+      | {| decl_name := na; decl_body := None; decl_type := ty |},
+        {| decl_name := na'; decl_body := None; decl_type := ty' |} => 
+        fun wtd wtd' =>
+        eqna <- check_eq_true (eqb_binder_annot na na') (Msg "Binder annotations do not match") ;;
+        cumt <- convert Γ ty ty' wtd wtd' ;;
+        ret (let 'sq cumt := cumt in sq _)      
+      | _, _ =>
+        fun wtd wtd' => raise (Msg "While checking cumulativity of contexts: declarations do not match")
+      end.
+    Next Obligation.
+      constructor; pcuics. now apply eqb_binder_annot_spec.
+    Qed.
+    Next Obligation.
+      constructor; pcuics. now apply eqb_binder_annot_spec.
+    Qed.
+
+    Lemma cumul_ctx_rel_close Γ Δ Δ' : 
+      cumul_ctx_rel Σ Γ Δ Δ' ->
+      cumul_context Σ (Γ ,,, Δ) (Γ ,,, Δ').
+    Proof.
+      induction 1; pcuic.
+    Qed.
+
+    Lemma conv_ctx_rel_close Γ Δ Δ' : 
+      conv_context_rel Σ Γ Δ Δ' ->
+      conv_context Σ (Γ ,,, Δ) (Γ ,,, Δ').
+    Proof.
+      induction 1; pcuic. simpl. constructor; eauto.
+      depelim p; constructor; auto.
+    Qed.
+
+    Lemma context_cumulativity_welltyped Γ Γ' t : 
+      welltyped Σ Γ t ->
+      cumul_context Σ Γ' Γ ->
+      wf_local Σ Γ' ->
+      welltyped Σ Γ' t.
+    Proof.
+      destruct HΣ.
+      intros [s Hs] cum wfΓ'; exists s; eapply context_cumulativity; eauto.
+    Qed.
+
+    Lemma context_conversion_welltyped Γ Γ' t : 
+      welltyped Σ Γ t ->
+      conv_context Σ Γ' Γ ->
+      wf_local Σ Γ' ->
+      welltyped Σ Γ' t.
+    Proof.
+      destruct HΣ.
+      intros [s Hs] cum wfΓ'; exists s; eapply context_conversion; eauto.
+      now eapply conv_context_sym.
+    Qed.
+    
+    Lemma context_cumulativity_wt_decl Γ Γ' d :
+      wt_decl Σ Γ d ->
+      cumul_context Σ Γ' Γ ->
+      wf_local Σ Γ' ->
+      wt_decl Σ Γ' d.
+    Proof.
+      destruct d as [na [b|] ty]; simpl;
+      intuition pcuics; eapply context_cumulativity_welltyped; pcuics.
+    Qed.
+    
+    Lemma context_conversion_wt_decl Γ Γ' d :
+      wt_decl Σ Γ d ->
+      conv_context Σ Γ' Γ ->
+      wf_local Σ Γ' ->
+      wt_decl Σ Γ' d.
+    Proof.
+      destruct d as [na [b|] ty]; simpl;
+      intuition pcuics; eapply context_conversion_welltyped; pcuics.
+    Qed.
+
+    Lemma cumul_decls_irrel_sec Γ Γ' d d' :
+      cumul_decls Σ Γ Γ d d' ->
+      cumul_decls Σ Γ Γ' d d'.
+    Proof.
+      intros cum; depelim cum; intros; constructor; auto.
+    Qed.
+    
+    Lemma conv_decls_irrel_sec Γ Γ' d d' :
+      conv_decls Σ Γ Γ d d' ->
+      conv_decls Σ Γ Γ' d d'.
+    Proof.
+      intros cum; depelim cum; intros; constructor; auto.
+    Qed.
+
+    Lemma inv_wf_local Γ d :
+      wf_local Σ (Γ ,, d) ->
+      wf_local Σ Γ * wt_decl Σ Γ d.
+    Proof.
+      intros wfd; depelim wfd; split; simpl; pcuic.
+      now exists t.
+    Qed.
+
+    Lemma cumul_ctx_rel_cons {Γ Δ Δ' d d'} (c : cumul_ctx_rel Σ Γ Δ Δ') 
+      (p : cumul_decls Σ (Γ,,, Δ) (Γ ,,, Δ') d d') : 
+      cumul_ctx_rel Σ Γ (Δ ,, d) (Δ' ,, d').
+    Proof.
+      destruct d as [na [b|] ty], d' as [na' [b'|] ty']; try constructor; auto.
+    Qed.
+    Lemma conv_ctx_rel_cons {Γ Δ Δ' d d'} (c : conv_context_rel Σ Γ Δ Δ') 
+      (p : conv_decls Σ (Γ,,, Δ) (Γ ,,, Δ') d d') : 
+      conv_context_rel Σ Γ (Δ ,, d) (Δ' ,, d').
+    Proof.
+      destruct d as [na [b|] ty], d' as [na' [b'|] ty']; try constructor; auto;
+      depelim p; constructor; auto.
+    Qed.
+
+    Program Fixpoint check_cumul_ctx Γ Δ Δ' 
+      (wfΔ : ∥ wf_local Σ (Γ ,,, Δ) ∥) (wfΔ' : ∥ wf_local Σ (Γ ,,, Δ') ∥) : 
+      typing_result (∥ cumul_ctx_rel Σ Γ Δ Δ' ∥) :=
+      match Δ, Δ' with
+      | [], [] => ret (sq All2_fold_nil)
+      | decl :: Δ, decl' :: Δ' => 
+        cctx <- check_cumul_ctx Γ Δ Δ' _ _ ;;
+        cdecl <- check_cumul_decl (Γ ,,, Δ) decl decl' _ _ ;;
+        ret _
+      | _, _ => raise (Msg "While checking cumulativity of contexts: contexts have not the same length")
+      end.
+      Next Obligation.
+        sq; now depelim wfΔ.
+      Qed.
+      Next Obligation.
+        sq; now depelim wfΔ'.
+      Qed.
+      Next Obligation.
+        sq.
+        depelim wfΔ; simpl.
+        destruct l; eexists; eauto.
+        destruct l; split; eexists; eauto.
+      Qed.
+      
+      Next Obligation.
+        pose proof HΣ as [wfΣ].
+        destruct wfΔ as [wfΔ], wfΔ' as [wfΔ'], cctx as [cctx].
+        assert(cumul_context Σ (Γ ,,, Δ) (Γ ,,, Δ')).
+        now apply cumul_ctx_rel_close.
+        simpl in *. eapply inv_wf_local in wfΔ as [wfΔ wfd].
+        eapply inv_wf_local in wfΔ' as [wfΔ' wfd'].
+        eapply context_cumulativity_wt_decl. 3:eassumption. all:pcuics.
+      Qed.
+      Next Obligation.
+        pose proof HΣ as [wfΣ].
+        destruct wfΔ as [wfΔ], wfΔ' as [wfΔ'], cctx as [cctx], cdecl as [cdecl].
+        constructor.
+        eapply inv_wf_local in wfΔ as [wfΔ wfd].
+        eapply inv_wf_local in wfΔ' as [wfΔ' wfd'].
+        apply cumul_ctx_rel_cons. auto.
+        eapply cumul_decls_irrel_sec; pcuics.
+      Qed.
+      Next Obligation.
+        split. intros. intros []. congruence. intros []; congruence.
+      Qed.
+      Next Obligation.
+        split. intros. intros []. congruence. intros []; congruence.
+      Qed.
+    
+    Program Fixpoint check_conv_ctx Γ Δ Δ' 
+      (wfΔ : ∥ wf_local Σ (Γ ,,, Δ) ∥) (wfΔ' : ∥ wf_local Σ (Γ ,,, Δ') ∥) : 
+      typing_result (∥ conv_context_rel Σ Γ Δ Δ' ∥) :=
+      match Δ, Δ' with
+      | [], [] => ret (sq All2_fold_nil)
+      | decl :: Δ, decl' :: Δ' => 
+        cctx <- check_conv_ctx Γ Δ Δ' _ _ ;;
+        cdecl <- check_conv_decl (Γ ,,, Δ) decl decl' _ _ ;;
+        ret _
+      | _, _ => raise (Msg "While checking convertibility of contexts: contexts have not the same length")
+      end.
+      Next Obligation.
+        sq; now depelim wfΔ.
+      Qed.
+      Next Obligation.
+        sq; now depelim wfΔ'.
+      Qed.
+      Next Obligation.
+        sq.
+        depelim wfΔ; simpl.
+        destruct l; eexists; eauto.
+        destruct l; split; eexists; eauto.
+      Qed.
+      
+      Next Obligation.
+        pose proof HΣ as [wfΣ].
+        destruct wfΔ as [wfΔ], wfΔ' as [wfΔ'], cctx as [cctx].
+        assert(conv_context Σ (Γ ,,, Δ) (Γ ,,, Δ')).
+        now apply conv_ctx_rel_close.
+        simpl in *. eapply inv_wf_local in wfΔ as [wfΔ wfd].
+        eapply inv_wf_local in wfΔ' as [wfΔ' wfd'].
+        eapply context_conversion_wt_decl. 3:eassumption. all:pcuics.
+      Qed.
+      Next Obligation.
+        pose proof HΣ as [wfΣ].
+        destruct wfΔ as [wfΔ], wfΔ' as [wfΔ'], cctx as [cctx], cdecl as [cdecl].
+        constructor.
+        eapply inv_wf_local in wfΔ as [wfΔ wfd].
+        eapply inv_wf_local in wfΔ' as [wfΔ' wfd'].
+        apply conv_ctx_rel_cons. auto.
+        eapply conv_decls_irrel_sec; pcuics.
+      Qed.
+      Next Obligation.
+        split. intros. intros []. congruence. intros []; congruence.
+      Qed.
+      Next Obligation.
+        split. intros. intros []. congruence. intros []; congruence.
+      Qed.
+       
   End InferAux.
 
   Program Definition lookup_ind_decl ind
@@ -257,6 +574,59 @@ Section Typecheck.
     destruct check_univs; auto.
   Qed.
 
+  Notation wt_brs Γ ci mdecl idecl p ps ptm ctors brs n := 
+    (All2i (fun i cdecl br =>
+      let brctxty := case_branch_type ci.(ci_ind) mdecl idecl p br ptm i cdecl in
+      ∥ (wf_local Σ (Γ ,,, br.(bcontext)) ×
+       conv_context Σ (Γ ,,, br.(bcontext)) (Γ ,,, brctxty.1)) ×
+      ((Σ ;;; Γ ,,, brctxty.1 |- br.(bbody) : brctxty.2) ×
+      (Σ ;;; Γ ,,, brctxty.1 |- brctxty.2 : tSort ps)) ∥) 
+      n ctors brs).
+  
+  Notation infer_ty :=
+    (forall (Γ : context) (HΓ : ∥ wf_local Σ Γ ∥) (t : term), typing_result ({ A : term & ∥ Σ ;;; Γ |- t : A ∥ })).
+
+  Section check_brs.
+    Context (infer : infer_ty)
+     (Γ : context) (wfΓ : ∥ wf_local Σ Γ ∥) (ps : Universe.t)
+     (ci : case_info) (mdecl : mutual_inductive_body)
+     (idecl : one_inductive_body) (p : predicate term) (ptm : term).
+     
+    Program Fixpoint check_branches (n : nat) (ctors : list constructor_body)
+       (brs : list (branch term)) {struct brs}
+       : typing_result (wt_brs Γ ci mdecl idecl p ps ptm ctors brs n) := 
+      match ctors, brs return typing_result (wt_brs Γ ci mdecl idecl p ps ptm ctors brs n) with
+      | [], [] => ret (All2i_nil : wt_brs Γ ci mdecl idecl p ps ptm [] [] n)
+      | cdecl :: cdecls, br :: brs =>
+        let brctxty := case_branch_type ci.(ci_ind) mdecl idecl p br ptm n cdecl in
+        check_br_ctx <- check_context_rel infer Γ br.(bcontext) wfΓ ;;
+        check_conv_ctx Γ br.(bcontext) brctxty.1 _ _ ;;
+        Z <- infer_cumul infer (Γ ,,, br.(bcontext)) _ br.(bbody) brctxty.2 _ ;;
+        X <- check_branches (S n) cdecls brs ;;
+        ret (t:=wt_brs Γ ci mdecl idecl p ps ptm (cdecl :: cdecls) (br :: brs) n) (All2i_cons _ X)
+      | [], _ :: _
+      | _ :: _, [] => raise (Msg "wrong number of branches")
+      end.
+
+      Next Obligation.
+        sq; now apply wf_local_app.
+      Defined.
+      Next Obligation.
+        clear infer. todo "case".
+      Defined.
+      Next Obligation.
+        clear infer. todo "case".
+      Defined.
+      Next Obligation.
+        clear infer. todo "case".
+      Defined.
+      Obligation Tactic := idtac.
+      Next Obligation.
+        intros.
+        clear infer. todo "case".
+      Defined.
+    End check_brs.
+
   Program Fixpoint infer (Γ : context) (HΓ : ∥ wf_local Σ Γ ∥) (t : term) {struct t}
     : typing_result ({ A : term & ∥ Σ ;;; Γ |- t : A ∥ }) :=
     match t with
@@ -320,55 +690,33 @@ Section Typecheck.
       | None => raise (UndeclaredConstructor ind k)
       end
 
-    | tCase (ind, par) p c brs =>
+    | tCase ci p c brs =>
       cty <- infer Γ HΓ c ;;
       I <- reduce_to_ind HΣ Γ cty.π1 _ ;;
       let '(ind'; I') := I in let '(u; I'') := I' in let '(args; H) := I'' in
-      check_eq_true (eqb ind ind')
+      check_eq_true (eqb ci.(ci_ind) ind')
                     (* bad case info *)
-                    (NotConvertible G Γ (tInd ind u) (tInd ind' u)) ;;
-      d <- lookup_ind_decl ind' ;;
-      let '(decl; d') := d in let '(body; HH) := d' in
-      check_coind <- check_eq_true (negb (isCoFinite (ind_finite decl)))
+                    (NotConvertible G Γ (tInd ci u) (tInd ind' u)) ;;
+      d <- lookup_ind_decl ci.(ci_ind) ;;
+      let '(mdecl; (idecl; isdecl)) := (d : ∑ (mdecl : mutual_inductive_body)
+          (idecl : one_inductive_body), declared_inductive _ _ _ _) in
+      check_coind <- check_eq_true (negb (isCoFinite (ind_finite mdecl)))
             (Msg "Case on coinductives disallowed") ;;
-      check_eq_true (ind_npars decl =? par)
+      check_eq_true (eqb (ind_npars mdecl) ci.(ci_npar))
                     (Msg "not the right number of parameters") ;;
-      IS <- infer_scheme infer Γ HΓ p ;;
-      let '(pctx; IS') := IS in let '(ps; typ_p) := IS' in
-      check_is_allowed_elimination ps (ind_kelim body);;
-      let pty := mkAssumArity pctx ps in
-      let params := firstn par args in
-      match build_case_predicate_type ind decl body params u ps with
-      | None => raise (Msg "failure in build_case_predicate_type")
-      | Some pty' =>
-        (* We could avoid one useless sort comparison by only comparing *)
-        (* the contexts [pctx] and [indctx] (what is done in Coq). *)
-        match iscumul Γ pty _ pty' _ with
-        | ConvError e => raise (NotCumulSmaller G Γ pty pty' pty pty' e)
-        | ConvSuccess =>
-          match map_option_out (build_branches_type ind decl body params u p) with
-          | None => raise (Msg "failure in build_branches_type")
-          | Some btys =>
-            let btyswf : ∥ All (isType Σ Γ ∘ snd) btys ∥ := _ in
-            (fix check_branches (brs btys : list (nat * term))
-              (HH : ∥ All (isType Σ Γ ∘ snd) btys ∥) {struct brs}
-                : typing_result
-                  (All2 (fun br bty => br.1 = bty.1 /\ ∥ Σ ;;; Γ |- br.2 : bty.2 ∥) brs btys)
-                        := match brs, btys with
-                           | [], [] => ret All2_nil
-                           | (n, t) :: brs , (m, A) :: btys =>
-                             W <- check_dec (Msg "not nat eq")
-                                           (EqDecInstances.nat_eqdec n m) ;;
-                             Z <- infer_cumul infer Γ HΓ t A _ ;;
-                             X <- check_branches brs btys _ ;;
-                             ret (All2_cons (conj _ _) X)
-                           | [], _ :: _
-                           | _ :: _, [] => raise (Msg "wrong number of branches")
-                           end) brs btys btyswf ;;
-              ret (mkApps p (List.skipn par args ++ [c]); _)
-          end
-        end
-      end
+      check_eq_true (eqb (ind_relevance idecl) ci.(ci_relevance))
+                    (Msg "invalid relevance annotation on case") ;;
+      wfpctx <- check_context_rel infer Γ p.(pcontext) HΓ ;;
+      let pctx := case_predicate_context ci.(ci_ind) mdecl idecl p in
+      check_wfpctx_conv <- check_conv_ctx Γ p.(pcontext) pctx _ _ ;;
+      retty <- infer_type infer (Γ ,,, p.(pcontext)) _ p.(preturn) ;;
+      let '(ps; typ_pret) := retty in
+      check_is_allowed_elimination ps (ind_kelim idecl);;
+      let ptm := it_mkLambda_or_LetIn pctx p.(preturn) in
+      let params := firstn ci.(ci_npar) args in
+      check_brs <- check_branches infer Γ HΓ ps ci mdecl idecl p ptm 
+        0 idecl.(ind_ctors) brs ;;
+       ret (mkApps ptm (List.skipn ci.(ci_npar) args ++ [c]); _)
 
     | tProj (ind, n, k) c =>
       d <- lookup_ind_decl ind ;;
@@ -529,14 +877,25 @@ Section Typecheck.
   Defined.
 
   (* tCase *)
-  Next Obligation. simpl; eauto using validity_wf. Qed.
-  Next Obligation. simpl; eauto using validity_wf. Qed.
+  Obligation Tactic := intros; Program.Tactics.destruct_conjs; cbn in *; subst.
+  Next Obligation. sq. eapply validity_term in X as []; eauto.
+    eexists; eauto using validity_wf. Defined.
+  Next Obligation. sq. now eapply wf_local_app. Defined.
+  Next Obligation. sq. eapply wf_local_app; auto. todo "case". Defined.
+  Next Obligation. sq. now eapply wf_local_app. Defined.
   Next Obligation.
-    destruct X1, X11. sq.
-    change (eqb ind I = true) in H0.
-    destruct (eqb_spec ind I) as [e|e]; [destruct e|discriminate].
-    change (eqb (ind_npars d) par = true) in H1.
-    destruct (eqb_spec (ind_npars d) par) as [e|e]; [|discriminate].
+    noconf Heq_anonymous. rename filtered_var into mdecl.
+    destruct H, X6, X7, X8.
+    noconf Heq_I; noconf Heq_I'; noconf Heq_I''.
+    noconf Heq_retty. sq. clear H H0 r r1.
+    rename X0 into idecl.
+    change (eqb ci.(ci_ind) I = true) in H1.
+    destruct (eqb_spec ci.(ci_ind) I) as [e|e]; [destruct e|discriminate].
+    change (eqb (ind_npars mdecl) ci.(ci_npar) = true) in H2.
+    destruct (eqb_spec (ind_npars mdecl) ci.(ci_npar)) as [e|e]; [|discriminate].
+    rewrite -e /ptm. 
+    todo "case".
+(*
     rename Heq_anonymous into HH. symmetry in HH.
     simpl in *.
     rewrite <- e in HH.
@@ -548,11 +907,37 @@ Section Typecheck.
     eapply validity in X; auto.
     eapply PCUICInductives.isType_it_mkProd_or_LetIn_inv in X; eauto.
     eapply isType_wf_universes in X; auto.
-    now exact (elimT wf_universe_reflect X).
-  Qed.
+    now exact (elimT wf_universe_reflect X).*)
+  Defined.
+  (* The obligation tactic removes useful lets here. *)
+  Obligation Tactic := idtac.
 
-  Next Obligation.
-    symmetry in Heq_anonymous1.
+  (*Next Obligation.
+    intros.
+    cbn. sq. splits.
+    - now eapply wf_local_app.
+    - now eapply conv_ctx_rel_close.
+    - eapply context_conversion; tea.
+      eapply wf_local_app; tas. todo "cases".
+      now eapply conv_ctx_rel_close.
+    - todo "cases".
+  Defined.*)
+  (*Next Obligation.
+    intros. cbn. subst filtered_var.
+    idtac; Program.Tactics.destruct_conjs. simpl proj1_sig in *.
+    cbn in *.
+    destruct X6, X8, H; noconf Heq_I; noconf Heq_I'; noconf Heq_I''.
+    noconf Heq_anonymous. noconf Heq_retty. destruct wfpctx as [wfpctx].
+    noconf H.
+    clear H H0. destruct X5 as [Hc]. sq. subst t.
+    change (eqb ci.(ci_ind) I = true) in H1.
+    destruct (eqb_spec ci.(ci_ind) I) as [e|e]; [destruct e|discriminate].
+    change (eqb (ind_npars d) ci.(ci_npar) = true) in H2.
+    destruct (eqb_spec (ind_npars d) ci.(ci_npar)) as [e|e]; [|discriminate].
+    todo "cases".
+    (* econstructor; eauto.
+    todo "case". branches *)
+    (*symmetry in Heq_anonymous1.
     unfold iscumul in Heq_anonymous1. simpl in Heq_anonymous1.
     apply isconv_term_sound in Heq_anonymous1.
     red in Heq_anonymous1.
@@ -578,22 +963,12 @@ Section Typecheck.
     have [pctx' da] : (∑ pctx', destArity [] pty' =  Some (pctx', X0)).
     { symmetry in Heq_anonymous0.
       unshelve eapply (PCUICInductives.build_case_predicate_type_spec (Σ.1, ind_universes d)) in Heq_anonymous0 as [parsubst [_ ->]].
-      eauto. eapply (PCUICWeakeningEnv.on_declared_inductive wfΣ) HH in as [? ?]. eauto.
+      eauto. eapply (PCUICWeakeningEnv.on_declared_inductive wfΣ) as [? ?]. eauto.
       eexists. rewrite !destArity_it_mkProd_or_LetIn; simpl. reflexivity. }
-    eapply PCUICInductiveInversion.build_branches_type_wt. 6:eapply typ_p. all:eauto.
-  Defined.
-
-  Next Obligation.
-    sq.
-    depelim HH; auto.
-  Defined.
-  Next Obligation.
-    sq.
-    depelim HH; auto.
-  Defined.
-
-  (* The obligation tactic removes a useful let here. *)
-  Obligation Tactic := idtac.
+    eapply PCUICInductiveInversion.build_branches_type_wt. 6:eapply typ_p. all:eauto.*)
+  Defined.*)
+  
+(*
   Next Obligation.
     intros. clearbody btyswf. idtac; Program.Tactics.program_simplify.
     symmetry in Heq_anonymous1.
@@ -628,11 +1003,11 @@ Section Typecheck.
     - destruct isCoFinite; auto.
     - symmetry; eauto.
   Defined.
-
+*)
   Obligation Tactic := Program.Tactics.program_simplify ; eauto 2.
 
   (* tProj *)
-  Next Obligation. simpl; eauto using validity_wf. Qed.
+  Next Obligation. simpl; eauto using validity_wf. Defined.
   Next Obligation.
     simpl in *; sq; eapply type_Proj with (pdecl := (i, t0)).
     - split. eassumption. split. symmetry; eassumption. cbn in *.
@@ -643,23 +1018,21 @@ Section Typecheck.
       eapply validity_term in X5; eauto.
       destruct (ssrbool.elimT (eqb_spec ind I)); auto.
       unshelve eapply (PCUICInductives.isType_mkApps_Ind _ X7 _) in X5 as [parsubst [argsubst [[sp sp'] cu]]]; eauto.
-      pose proof (PCUICContexts.context_subst_length2 (PCUICSpine.inst_ctx_subst sp)).
-      pose proof (PCUICContexts.context_subst_length2 (PCUICSpine.inst_ctx_subst sp')).
+      pose proof (PCUICContextSubst.context_subst_length2 (PCUICSpine.inst_ctx_subst sp)).
+      pose proof (PCUICContextSubst.context_subst_length2 (PCUICSpine.inst_ctx_subst sp')).
       autorewrite with len in H, H2.
-      destruct (PCUICWeakeningEnv.on_declared_inductive HΣ X7) eqn:ond.
+      destruct (on_declared_inductive X7) eqn:ond.
       rewrite -o.(onNpars) -H.
       forward (o0.(onProjections)).
       intros H'; rewrite H' nth_error_nil // in Heq_anonymous.
-      destruct ind_cunivs as [|cs []]; auto.
+      destruct ind_ctors as [|cs []]; auto.
       intros onps.
       unshelve epose proof (onps.(on_projs_noidx _ _ _ _ _ _)).
-      rewrite ond /= in H2.
-      change (ind_indices o0) with (ind_indices o0) in *.
-      destruct (ind_indices o0) => //.
+      destruct (ind_indices X6) => //.
       simpl in H2.
       rewrite List.skipn_length in H2.
       rewrite List.firstn_length. lia.
-  Qed.
+  Defined.
 
   (* tFix *)
   Next Obligation. sq. constructor; auto. exists W; auto. Defined.
@@ -675,7 +1048,7 @@ Section Typecheck.
   Next Obligation.
     clear -XX HΣ. sq.
     now depelim XX.
-  Qed.
+  Defined.
   Next Obligation.
     assert (∥ All (fun d => ((Σ;;; Γ ,,, fix_context mfix |- dbody d : (lift0 #|fix_context mfix|) (dtype d)))%type) mfix ∥). {
       eapply All_sq, All_impl.  exact YY.
@@ -707,33 +1080,6 @@ Section Typecheck.
     symmetry; eassumption.
   Qed.
 
-  Lemma sq_wfl_nil : ∥ wf_local Σ [] ∥.
-  Proof.
-   repeat constructor.
-  Qed.
-
-  Program Fixpoint check_context Γ : typing_result (∥ wf_local Σ Γ ∥)
-    := match Γ with
-       | [] => ret sq_wfl_nil
-       | {| decl_body := None; decl_type := A |} :: Γ =>
-         HΓ <- check_context Γ ;;
-         XX <- infer_type infer Γ HΓ A ;;
-         ret _
-       | {| decl_body := Some t; decl_type := A |} :: Γ =>
-         HΓ <- check_context Γ ;;
-         XX <- infer_type infer Γ HΓ A ;;
-         XX <- infer_cumul infer Γ HΓ t A _ ;;
-         ret _
-       end.
-  Next Obligation.
-    sq. econstructor; tas. econstructor; eauto.
-  Qed.
-  Next Obligation.
-    sq. econstructor; tea.
-  Qed.
-  Next Obligation.
-    sq. econstructor; tas. econstructor; eauto.
-  Qed.
 
 (* 
   Program Definition check_isWfArity Γ (HΓ : ∥ wf_local Σ Γ ∥) A
